\documentclass[10pt]{homeworg}

\title{Homework 1}
\author{Kevin Yang}


\begin{document}

\maketitle

\exercise
Let $X = (x_1, x_2, \ldots, x_n)$ \\
\vspace{0.5cm}
$x_i \sim Pois(\lambda)$  \hspace{2cm} $\lambda \sim \Gamma(\alpha, \beta)$
\\
We have that:
\begin{align*}
P(\lambda \mid X) &= \frac{P(X \mid \lambda)P(\lambda)}{P(X)}\\
				  &\propto P(X \mid \lambda)P(\lambda)\\
				  &\propto \lambda^{n\bar{x}}e^{-n\lambda}\lambda^{\alpha-1}e^{-\beta\lambda}\\
				  &= \lambda^{n\bar{x}+\alpha-1}e^{-(n+\beta)\lambda}
\end{align*}

Therefore, $P(\lambda \mid X) \sim \Gamma(n\bar{x}+\alpha, \beta+n)$ and the Gamma distribution is conjugate to the Poisson distribution.

\exercise
Let $s = (s_1, s_2, \ldots, s_n)$, $s' = (s_1', s_2', \ldots, s_n')$ and $s_{-i} = (s_1, \ldots, s_{i-1}, s_{i+1}, \ldots, s_n)$\\
Detailed balance equation: $\pi(s)P(s,s')=\pi(s')P(s',s)$\\

w.l.g consider an update for $s_1$\\
\vspace{0.5cm}

\textit{Case 1:} $s_{-1} \neq s_{-1}'$
\begin{align*}
\pi(s)P(s,s') = \pi(s')P(s',s) = 0
\end{align*}


\textit{Case 2:} $s_{-1} = s_{-1}'$
\begin{align*}
\pi(s)P(s,s') &= \pi(s)P(s_1' \mid s_{-1}')\\
			  &= \pi(s)\frac{\pi(s')}{\sum_z \pi(z, s_{-1}')}\\
			  &= \pi(s')\frac{\pi(s)}{\sum_z \pi(z, s_{-1})}\\
			  &= \pi(s')P(s_1 \mid s_{-1})\\
			  &= \pi(s')P(s',s)
\end{align*}

Consider the move from $s$ to $s'$. The acceptance probability for MH will be

\begin{align*}
\frac{\pi(s')P(s',s)}{\pi(s)P(s,s')}
\end{align*}

We have that

\begin{align*}
\frac{P(s',s)}{P(s,s')} &= \frac{\frac{\pi(s)}{\sum_z \pi(z,s_{-1})}}{\frac{\pi(s')}{\sum_z \pi(z, s_{-1}')}}\\
					   &= \frac{\pi(s)}{\pi(s')}
\end{align*}

So

\begin{align*}
\frac{\pi(s')P(s',s)}{\pi(s)P(s,s')} = \frac{\pi(s')\pi(s)}{\pi(s)\pi(s')} = 1
\end{align*}

\end{document}